\documentclass[12pt]{article}
\usepackage[a4paper, margin=0.75in]{geometry}
\usepackage[document]{ragged2e}
\usepackage{graphicx}
\graphicspath{ {./images/} }
\input{preamble.tex}
\usepackage[scr]{rsfso}
\usepackage{physics}
\usepackage{multicol}
\renewcommand{\arraystretch}{2.5}

\newcommand{\Lap}{\mathscr{L}}

\title{
    \textbf{Laplace Transform}
}

\author{
    Turja Roy\\
    ID: 2108052
}
\date{}

\begin{document}
\maketitle
\tableofcontents
\newpage

%%%%%%%%%%%%%%%%%%%%%%%%%%%%%%%%%%%%%%%%%%%%%%%%%
%  Definition, Existence, and Basic Properties  %
%%%%%%%%%%%%%%%%%%%%%%%%%%%%%%%%%%%%%%%%%%%%%%%%%

\section{Definition, Existence, and Basic Properties of the Laplace Transform}

%%%%%%%%%%%%%%%%%%%%%%%%%%%%%%
%  Definition and Existence  %
%%%%%%%%%%%%%%%%%%%%%%%%%%%%%%

\subsection{Definition and Existence}

\begin{definition}{Laplace Transform}{}
    Let $F$ be a real-valued function of the real variable $t$, defined for $t>0$. Let $s$ be a variable that we shall assume to be real, and consider the function $f$ defined by
    \begin{equation} \label{eq1}
        f(s) = \int_{0}^{\infty} {e^{-st} F(t)} \: d{t} 
    \end{equation}
    for all values of $s$ for which this integral exists. The function $f$ defined by the integral \eqref{eq1} is called the Laplace Transform of the function $F$. We shall denote the Laplace transform of $F$ by $\Lap\{F(t)\}$.\\
    Thus the Laplace transform of a function $f$ is given by
    \begin{equation} \label{eq2}
        \Lap\{ F(t) \} = f(s) = \int_{0}^{\infty} {e^{-st} F(t)} \: d{t}  = \lim_{R \to \infty} \int_{0}^{R} {e^{-st} F(t)} \: d{t} 
    \end{equation}
\end{definition}

Some ways to write Laplace transforms:\\
\[ \Lap{F(t)} = f(s) = \int_{0}^{\infty} { e^{-st} F(t) } \: d{t} \]
\[ \Lap{G(t)} = g(s) \]
\[ \Lap{u(t)} = \tilde{u}(s) \]

\vspace{20pt}
\begin{table}[htpb]
    \centering

    \begin{tabular}{c | c}
        \hline
        $F(t)$ &  $\Lap\{ F(t) \} = f(s)$ \\
        \hline\hline
        $1$ & $\dfrac{1}{s}$ \\\hline
        $t$ & $\dfrac{1}{s^2}$ \\\hline
        $e^{at}$ & $\dfrac{1}{s-a}$ \\\hline
        $\sin{at}$ & $\dfrac{a}{s^2+a^2}$ \\\hline
        $\cos{at}$ & $\dfrac{s}{s^2+a^2}$ \\
        \hline
    \end{tabular}
    \begin{tabular}{c | c}
        \hline
        $F(t)$ &  $\Lap\{ F(t) \} = f(s)$ \\
        \hline\hline
        $n$ & $\dfrac{n}{s}$ \\\hline
        $t^n$ &  $\dfrac{n!}{s^{n+1}}$ \\\hline
        $e^{-at}$ & $\dfrac{1}{s+a}$ \\\hline
        $\sinh{at}$ & $\dfrac{a}{s^2-a^2}$ \\\hline
        $\cosh{at}$ &  $\dfrac{s}{s^2-a^2}$ \\
        \hline
    \end{tabular}

    \caption{Functions and their Laplace Transform}
    \label{LapTable}
\end{table}

\newpage
\begin{multicols}{2}
    [
    \underline{\textbf{Proofs :}}\\
    ]
    Let $F(t) = n$, for $t>0$\\
    Then\\
    \begin{align*}
        \Lap \{ n \} &= \int_{0}^{\infty} { e^{-st} \cdot n } \: d{t} \\
                     &= \eval{ n\frac{-e^{st}}{s} }_{0}^{\infty} \\
                     &= \frac{n}{s}\qed
    \end{align*}\\
    \columnbreak

    Let $F(t) = t$, for $t>0$\\
    Then\\
    \begin{align*}
        \Lap \{ t \} &= \int_{0}^{\infty} { e^{-st} \cdot t } \: d{t} \\
                     &= -t \frac{e^{-st}}{s} + \int_{0}^{\infty} {\frac{e^{-st}}{s}} \: d{t} \\
                     &= -e^{-st}\frac{t}{s}\bigg|_{0}^{\infty} - e^{-st}\frac{1}{s^2}\bigg|_{0}^{\infty} \\
                     &= \frac{1}{s^2}\qed
    \end{align*}
\end{multicols}

\vspace{20pt}
Let $F(t) = t^{n}$, for $t>0$ \\
Then\\
\begin{align*}
    \Lap \{ t^{n} \} &= \int_{0}^{\infty} {e^{-s t}t^n} \: d{t} \\
                     &= -t^n \frac{e^{s t}}{s} + \int_{0}^{\infty} { nt^{n-1} \frac{e^{-s t}}{s} } \: d{t} \\
                     &= \eval{ -nt^{n-1} \frac{e^{-s t}}{s^2} }_{0}^{\infty} + \int_{0}^{\infty} { n(n-1)t^{n-2} \frac{e^{-s t}}{s^2} } \: d{t} \\
                     &= \eval{ -n(n-1)t^{n-2} \left( \frac{e^{-s t}}{s^3} \right) }_{0}^{\infty} + \int_{0}^{\infty} { n(n-1)(n-2)t^{n-3} \frac{e^{-s t}}{s^3} } \: d{t}  \\
                     &= \cdots \\
                     &= \eval{n!t^{n-n}\frac{e^{-s t}}{s^{n+1}}}_{0}^{\infty} + \int_{0}^{\infty} { n(n-1)\cdots(n-n) \frac{e^{-s t}}{s^{n+1}} } \: d{t} \\
                     &= \frac{n!}{s^{n+1}}\qed
\end{align*}\\~\\

\begin{multicols}{2}
    Let $F(t) = e^{at}$, for $t>0$\\
    Then\\
    \begin{align*}
        \Lap \{ e^{at} \} &= \int_{0}^{\infty} { e^{-s t} e^{at} } \: d{t} \\
                          &= \int_{0}^{\infty} { e^{(a-s)t} } \: d{t} \\
                          &= \eval{ \frac{e^{(a-s)t}}{a-s} }_{0}^{\infty} \\
                          &= \frac{1}{s-a}\qed
    \end{align*}
    \columnbreak
    
    Let $F(t)=e^{-at}$, for $t>0$ \\
    Then\\
    \begin{align*}
        \Lap \{ e^{-at} \} &= \int_{0}^{\infty} {e^{-s t} e^{-at}} \: d{t} \\
        &= \int_{0}^{\infty} {e^{-(a+s)t}} \: d{x} \\
        &= \eval{ \frac{e^{-(a+s)t}}{s+a} }_{0}^{\infty} \\
        &= \frac{1}{s+a}\qed
    \end{align*}
\end{multicols}

\newpage
\begin{multicols}{2}
    Let $F(t) = \sin{at}$, for $t>0$ \\
    Then\\
    \begin{align*}
        \Lap \{ \sin{at} \} &= \int_{0}^{\infty} { e^{-s t \sin{at}} } \: d{t} \\
        &= - \eval{ \frac{e^{-s t}}{s^2+a^2} \left( s\sin{at} + a\cos{at} \right) }_{0}^{\infty} \\
        &= \frac{a}{s^2+a^2}\qed
    \end{align*}
    \columnbreak
    
    Let $F(t) = \cos{at}$, for $t>0$ \\
    Then\\
    \begin{align*}
        \Lap \{ \cos{at} \} &= \int_{0}^{\infty} { e^{-s t}\cos{at} } \: d{t} \\
        &= \eval{ \frac{e^{-s t}}{s^2+a^2} \left( -s\cos{at} + a\sin{at} \right) }_{0}^{\infty} \\
        &= \frac{s}{s^2+a^2}\qed
    \end{align*}
\end{multicols}


\vspace{30pt}
\begin{theorem}{}{}
    \textbf{Hypothesis: } Let $F$ be a real function that has the following properties:
    \begin{enumerate}
        \item $F$ is a piecewise continuous in every finite closed interval $0 \le t \le a \: (b>0)$.
        \item $F$ is of exponential order, i.e, there exists $\alpha$, $M>0$, and $t_0>0$ such that
    \end{enumerate}
    \[ e^{-\alpha t}|F(t)| < M \text{ for } t>t_0 \]
    
    \textbf{Conclusion: } The Laplace transform of $F$ exists for $s>\alpha$.
    \[
        \Lap \{ F(t) \} = \int_{0}^{\infty} {e^{-s t}F(t)} \: d{t}
    \] 
\end{theorem}


%%%%%%%%%%%%%%%%%%%%%%%%%%%%%%%%%%%%%%%%%%%%%%%
%  Basic Properties of the Laplace Transform  %
%%%%%%%%%%%%%%%%%%%%%%%%%%%%%%%%%%%%%%%%%%%%%%%
\vspace{30pt}
\subsection{Basic Properties of the Laplace Transform}

\begin{theorem}{The Linear Property}{}
    \\Let $F_1$ and $F_2$ be functions whose Laplace transform exist, and let $c_1$ and $c_2$ be constants. Then
    \[
        \Lap \{ c_1F_1(t) + c_2F_2(t) \} = c_1 \Lap \{ F_1(t) \} + c_2 \Lap \{ F_2(t) \}
    \]
\end{theorem}

\begin{example}{
        $$ \Lap \{ 4t^2 - 3\cos{2t} + 5e^{-t} \} $$
    }{}
    \begin{align*}
        \Lap \{ 4t^2 - 3\cos{2t} + 5e^{-t} \} &= 4 \Lap \{ t^2 \} - 3 \Lap \{ \cos{2t} \} + 5 \Lap \{ e^{-t} \} \\
        &= 4 \cdot \frac{2!}{s^3} - 3 \cdot \frac{s}{s^2+4} + 5 \cdot \frac{1}{s+1} \\
        &= \frac{8}{s^3} - \frac{3s}{s^2+4} + \frac{5}{s+1}
    \end{align*}
\end{example}

\begin{theorem}{First translation of Shifting property}{}
    \\If \[
        \Lap \{ F(t) \} = f(s)
    \] then
    \[ \Lap \{ e^{at}F(t) \} = f(s-a) \]
\end{theorem}

\begin{example}{\[
    \Lap \{ e^{-t}\cos{2t} \}
\]}{}
    Since $\Lap \{ \cos{2t} \} = \dfrac{s}{s^2+4}$, we have
    \[
        \Lap \{ e^{-t}\cos{2t} = \frac{s+1}{(s+1)^2 + 4} = \frac{s+1}{s^2+2s+5} \}
    \]
\end{example}

\begin{theorem}{Second translation or Shifting property}{}
    \\If \[
        \Lap \{ F(t) \} = f(s)
    \] and \[
        G(t) = 
        \begin{cases}
            F(t-a) & \text{for } t>a \\
            0 & \text{for } t < a
        \end{cases}
    \] then
    \[
        \Lap \{ G(t) \} = e^{-as}f(s)
    \]

\end{theorem}

\begin{example}{
        Find $\Lap \{ G(t) \}$ where $
        G(t) = 
        \begin{cases}
            \cos{t - \frac{2\pi}{3}} & \text{for } t > \frac{2\pi}{3} \\
            0 & \text{for } t < \frac{2\pi}{3}
        \end{cases}
        $
    }{}
    \begin{align*}
        \Lap \{ G(t) \} &= e^{-\frac{2\pi}{3}s} \cdot \Lap \{ \cos{t} \} \\
        &= e^{-\frac{2\pi}{3}s} \cdot \frac{s}{s^2+1} \\
        &= \frac{s e^{-\frac{2\pi}{3}s}}{s^2+1} \\
    \end{align*}
\end{example}

\begin{theorem}{Change of scale property}{}
    \\If \[
        \Lap \{ F(t) \} = f(s)
    \] then \[
        \Lap \{ F(at) \} = \frac{1}{a} f \left( \frac{s}{a} \right)
    \]
\end{theorem}

\begin{example}{Evaluate $\Lap \{ \sin{3t} \}$}{}
    \begin{align*}
        \Lap \{ \sin{3t} \} &= \frac{1}{3} \cdot \frac{1}{\left( \frac{s}{3} \right) + 1} \\
        &= \frac{1}{3} \cdot \frac{3^2}{s^2+3^2}\\
        &= \frac{3}{s^2+9}
    \end{align*}
\end{example}

\begin{theorem}{Multiplication by $t^n$}{}
    \\If \[
        \Lap \{ F(t) \} = f(s)
    \] then \[
        \Lap \{ t^nF(t) \} = (-1)^n \frac{d^n}{ds^n} f(s)
    \]
\end{theorem}

\begin{example}{Find $\Lap \{ t^2 \cos{at} \}$}{}
    \begin{align*}
        \Lap \{ t^2 \cos{at} \} &= (-1)^2 \cdot \frac{d^2}{d{x^2}} \: \left( \frac{s}{s^2 + a^2} \right) \\
        &= \dv{ \left[ \frac{s^2 + a^2 - 2s^2}{ (s^2 + a^2)^2 } \right] }{s} \\
        &= \dv{ \left[ \frac{a^2 - s^2}{(s^2 + a^2)^2} \right] }{s} \\
        &= \frac{(s^2+a^2)^2(-2s) - (-s^2+a^2)2(s^2+a^2)\cdot2s}{(s^2+a^2)^4} \\
        &= \frac{2s^3 - 6a^2s}{(s^2+a^2)^3}
    \end{align*}
\end{example}

\begin{theorem}{Division by $t$}{}
    \\If \[
        \Lap \{ F(t) \} = f(s)
    \] then \[
        \Lap \left\{ \frac{F(t)}{t} \right\} = \int_{s}^{\infty} {f(x)} \: d{x}
    \]
\end{theorem}

\begin{example}{Find $\Lap \{ \frac{\sin{t}}{t} \}$}{}
    \begin{align*}
        \Lap \left\{ \frac{\sin{t}}{t} \right\} &= \int_{s}^{\infty} {\frac{1}{s^2+1}} \: d{u} \\
        &= \tan^{-1}{u} \bigg|_s^\infty \\
        &= \frac{\pi}{2} - \tan^{-1}{s} = \cot^{-1}{s} \\
        &= \tan^{-1}{\frac{1}{s}}
    \end{align*}
\end{example}

\begin{theorem}{Laplace transform of Integral}{}
    \\If \[
        \Lap \{ F(t) \} = f(s)
    \] then \[
        \Lap \left\{ \int_{0}^{t} {F(x)} \: d{x} \right\} = \frac{1}{s} f(s)
    \]
\end{theorem}

\begin{example}{Evaluate $\Lap \{ \int_{0}^{t} {\frac{\sin{u}}{u}} \: d{u} \}$}{}
\[ \Lap \left\{ \frac{\sin{u}}{u} \right\} = \tan^{-1}{\frac{1}{s}} \]
    \[
        \Lap \left\{ \int_{0}^{t} {\frac{\sin{u}}{u}} \: d{u} \right\} = \frac{f(s)}{s} = \frac{1}{s} \tan^{-1}{\frac{1}{s}}
    \]
\end{example}

\begin{example}{Evaluate $\Lap \{ \int_{0}^{t} {\frac{\sin{u}}{u}} \: d{u} \}$}{}
    Let $F(t) = \frac{\sin{t}}{t}$
    \begin{align*}
        \Lap \left\{ \frac{\sin{t}}{t} \right\} &= \int_{s}^{\infty} {\frac{1}{u^2+1}} \: d{u} \\
         &= \tan^{-1}{u} \bigg|_s^\infty \\
         &= \tan^{-1}{\frac{1}{s}}
    \end{align*}
    \[
        \therefore \Lap \left\{ \int_{0}^{t} {\frac{\sin{u}}{u}} \: d{u} \right\} &= \frac{1}{s} \cdot \tan^{-1}{\frac{1}{s}} \\
        
    \]
\end{example}

\begin{example}{Evaluate $\Lap \{ \int_{0}^{t} {\sin{2u}} \: d{u} \}$}{}
    \[ \Lap \{ \sin{2t} \} = \frac{2}{s^2+4} \]
    \[ \therefore \Lap \left\{ \int_{0}^{t} {\sin{2u}} \: d{u} \right\} = \frac{2}{s^3 + 4s} \]
\end{example}

\begin{theorem}{Periodic functions}{}
    \\If \[
        \Lap \{ F(t) \} = f(s)
    \] then \[
        \Lap \{ F(t) \} = \frac{1}{1-e^{-Ts}} \int_{0}^{T} {e^{-st}F(t)} \: d{t}
    \] where $T$ is the period of $F(t)$.
\end{theorem}

\begin{example}{
        Find $\Lap \{ F(t) \}$ for \[
            F(t) = 
            \begin{cases}
                \sin{t} & \text{for } 0 < t < \pi \\
                0 & \text{for } \pi < t < 2\pi
            \end{cases}
        \]
    }{}
    \begin{align*}
        \Lap \{ F(t) \} &= \frac{1}{1 - e^{-2\pi s}} \int_{0}^{2\pi} { e^{st} \sin{t} } \: d{t} \\
        &= \frac{1}{1-e^{-2\pi s}} \int_{0}^{\pi} {e^{-st} \sin{t}} \: d{t}
    \end{align*}
\end{example}

\begin{example}{Find $\Lap \{ F(t) \}$ for \[
    F(t) =
    \begin{cases}
        t & \text{for } 0 < t < 1 \\
        0 & \text{for } 1 < t < 2
    \end{cases}
\]}{}
    \begin{align*}
        \Lap \{ F(t) \} &= \frac{1}{1-e^{-2s}} \int_{0}^{1} {t} \: d{t} \\
        &= \frac{t^2 \bigg|_0^1}{2 - 2e^{-2s}} \\
        &= \frac{1}{2 - 2e^{-2s}}
    \end{align*}
\end{example}

\begin{theorem}{Laplace transform of derivatives}{}
    \\If \[
        \Lap \{ F(t) \} = f(s)
    \] then \[
        \Lap \{ F'(t) \} = sf(s) - F(0)
    \] \[
        \Lap \{ F''(t) \} = s^2F(s) - sF(0) - F'(0)
    \] \[
        \Lap \{ F'''(t) = s^3f(s) - s^2F(0) - sF'(0) - F''(0) \}
    \] \[
        \boxed{ \Lap \{ F^{(n)}(t) \} = s^nf(s) - s^{n-1}F(0) - s^{n-2}F'(0) - \cdots - F^{(n-1)}(0) }
    \] \[
        \boxed{ \Lap \{ F^{(n)}(t) \} = s^nf(s) - \sum_{i=n-1}^{0}\sum_{j=0}^{n-1} s^i F^{(j)}(0) }
    \]
\end{theorem}

\begin{example}{}{}
    
\end{example}














\end{document}
